src/Lean/Meta/Tactic/Grind/AC/Eq.lean
@@ -9,6 +9,7 @@ public import Lean.Meta.Tactic.Grind.AC.Util
 import Lean.Meta.Tactic.Grind.AC.DenoteExpr
 import Lean.Meta.Tactic.Grind.AC.Proof
 import Lean.Meta.Tactic.Grind.AC.Seq
+import Lean.Meta.Tactic.Grind.AC.Inv
 public section
 namespace Lean.Meta.Grind.AC
 open Lean.Grind
@@ -79,6 +80,18 @@ def EqCnstr.eraseDup (c : EqCnstr) : ACM EqCnstr := do
   else
     return { c with lhs, rhs, h := .erase_dup c }
 
+def EqCnstr.erase0 (c : EqCnstr) : ACM EqCnstr := do
+  unless (← hasNeutral) do return c
+  let lhs := c.lhs.erase0
+  let rhs := c.rhs.erase0
+  if c.lhs == lhs && c.rhs == rhs then
+    return c
+  else
+    return { c with lhs, rhs, h := .erase0 c }
+
+def EqCnstr.cleanup (c : EqCnstr) : ACM EqCnstr := do
+  (← c.eraseDup).erase0
+
 def EqCnstr.orient (c : EqCnstr) : EqCnstr :=
   if compare c.rhs c.lhs == .gt then
     { c with lhs := c.rhs, rhs := c.lhs, h := .swap c }
@@ -127,16 +140,16 @@ private def simplifyRhsWithA (c : EqCnstr) (c' : EqCnstr) (r : AC.SubseqResult) 
 
 /-- Simplifies `c` using the basis when `(← isCommutative)` is `false` -/
 private def EqCnstr.simplifyA (c : EqCnstr) : ACM EqCnstr := do
-  let mut c ← c.eraseDup
+  let mut c ← c.cleanup
   repeat
     incSteps
     if (← checkMaxSteps) then return c
     if let some (c', r) ← c.lhs.findSimpA? then
       c := simplifyLhsWithA c c' r
-      c ← c.eraseDup
+      c ← c.cleanup
     else if let some (c', r) ← c.rhs.findSimpA? then
       c := simplifyRhsWithA c c' r
-      c ← c.eraseDup
+      c ← c.cleanup
     else
       trace[grind.debug.ac.simplify] "{← c.denoteExpr}"
       return c
@@ -178,16 +191,16 @@ private def simplifyWithAC' (c : EqCnstr) (c' : EqCnstr) : Option EqCnstr := do
 
 /-- Simplify `c` using the basis when `(← isCommutative)` is `true` -/
 private def EqCnstr.simplifyAC (c : EqCnstr) : ACM EqCnstr := do
-  let mut c ← c.eraseDup
+  let mut c ← c.cleanup
   repeat
     incSteps
     if (← checkMaxSteps) then return c
     if let some (c', r) ← c.lhs.findSimpAC? then
       c := simplifyLhsWithAC c c' r
-      c ← c.eraseDup
+      c ← c.cleanup
     else if let some (c', r) ← c.rhs.findSimpAC? then
       c := simplifyRhsWithAC c c' r
-      c ← c.eraseDup
+      c ← c.cleanup
     else
       trace[grind.debug.ac.simplify] "{← c.denoteExpr}"
       return c
@@ -272,5 +285,22 @@ def processNewDiseqImpl (a b : Expr) : GoalM Unit := withExprs a b do
   let eb ← asACExpr b
   let rhs ← norm eb
   { lhs, rhs, h := .core a b ea eb : DiseqCnstr }.assert
+
+def checkStruct : ACM Bool := do
+  -- TODO
+  return false
+
+def check : GoalM Bool := do profileitM Exception "grind ac" (← getOptions) do
+  if (← checkMaxSteps) then return false
+  let mut progress := false
+  checkInvariants
+  try
+    for opId in *...(← get').structs.size do
+      let r ← ACM.run opId checkStruct
+      progress := progress || r
+      if (← isInconsistent) then return true
+    return progress
+  finally
+    checkInvariants
 
 end Lean.Meta.Grind.AC
